src/panWeakestPreconditionScript.sml
@@ -4,388 +4,211 @@
 
 Theory panWeakestPrecondition
 Ancestors panReducedSem panReducedProps panPredicate
-
-fun elim_cases xs = EVERY (map (fn x => Cases_on x >> gvs[]) xs);
-
-Theorem state_clock_idem:
-  ∀s. s with clock := s.clock = s
-Proof
-  rw[state_component_equality]
-QED
+Libs BasicProvers
 
 Definition hoare_def:
-  hoare P prog Q ⇔ clkfree_p P ∧
-                   clkfree_q Q ∧
-                   ∀s. P s ⇒ ∃k. let (r,t) = evaluate (prog,s with clock := k)
-                                 in r ≠ SOME Error ∧
-                                    r ≠ SOME TimeOut ∧
-                                    Q (r,t)
+  hoare P prog Q ⇔ ∀s. P s ⇒ let (r,t) = evaluate (prog,s)
+                             in r ≠ SOME Error ∧ Q (r,t) ∨ r = SOME TimeOut
 End
 
 Theorem hoare_monotonic_p:
   ∀P P' prog Q. (∀s. P s ⇔ P' s) ⇒ (hoare P prog Q ⇔ hoare P' prog Q)
 Proof
   rw[hoare_def]
-  >> iff_tac
-  >> rw[]
-  >> drule clkfree_p_monotonic
-  >> gvs[]
 QED
 
 Definition wp_def:
-  wp prog Q s ⇔ clkfree_q Q ∧
-                ∃k. let (r,t) = evaluate (prog,s with clock := k)
-                    in r ≠ SOME Error ∧
-                       r ≠ SOME TimeOut ∧
-                       Q (r,t)
+  wp prog Q s ⇔ let (r,t) = evaluate (prog,s)
+                    in r ≠ SOME Error ∧ Q (r,t) ∨ r = SOME TimeOut
 End
 
-Theorem wp_clkfree:
-  ∀prog Q. clkfree_p (wp prog Q)
-Proof
-  rw[clkfree_p_def,wp_def]
-QED
-
 Theorem wp_is_weakest_precondition:
-  ∀P prog Q. clkfree_p P ∧ clkfree_q Q ⇒ hoare (wp prog Q) prog Q ∧
-                                         (hoare P prog Q ⇔ (∀s. P s ⇒ wp prog Q s))
+  ∀P prog Q. hoare (wp prog Q) prog Q ∧ (hoare P prog Q ⇔ (∀s. P s ⇒ wp prog Q s))
 Proof
-  metis_tac[hoare_def,wp_def,wp_clkfree]
+  rw[hoare_def,wp_def]
 QED
 
 Theorem wp_monotonic:
-  ∀A B prog. (clkfree_q A ∧ clkfree_q B) ⇒ (∀s. A s ⇒ B s) ⇒ (∀s. wp prog A s ⇒ wp prog B s)
+  ∀A B prog. (∀s. A s ⇒ B s) ⇒ (∀s. wp prog A s ⇒ wp prog B s)
 Proof
   rw[wp_def,hoare_def]
   >> pairarg_tac
-  >> qexists ‘k’
   >> gvs[]
 QED
 
 Theorem wp_conj:
-  ∀A B p. clkfree_q A ∧ clkfree_q B ⇒ (∀s. wp p (λ(r,t). A (r,t) ∧ B (r,t)) s ⇔ wp p A s ∧ wp p B s)
+  ∀A B p s. wp p (λ(r,t). A (r,t) ∧ B (r,t)) s ⇔ wp p A s ∧ wp p B s
 Proof
   rw[wp_def]
   >> iff_tac
   >> rw[]
-  >- (qexists ‘k’ >> pairarg_tac >> gvs[])
-  >- (qexists ‘k’ >> pairarg_tac >> gvs[])
-  >- metis_tac[clkfree_q_conj]
-  >> Cases_on ‘k > k'’
-  >> rpt (pairarg_tac >> gvs[])
-  >> gvs[clkfree_q_def]
-  >- (qexists ‘k’
-      >> qspecl_then [‘p’, ‘s with clock := k'’, ‘r’, ‘t’, ‘k - k'’]
-                     assume_tac evaluate_add_clock_eq
-      >> first_x_assum $ (qspecl_then [‘r’, ‘t’, ‘t.clock’, ‘k + t.clock - k'’] assume_tac)
-      >> gvs[state_clock_idem])
-  >> qexists ‘k'’
-  >> qspecl_then [‘p’, ‘s with clock := k’, ‘r'’, ‘t'’, ‘k' - k’]
-                 assume_tac evaluate_add_clock_eq
-  >> last_x_assum $ (qspecl_then [‘r’, ‘t'’, ‘t'.clock’, ‘k' + t'.clock - k’] assume_tac)
-  >> gvs[state_clock_idem]
-QED
-
-Theorem wp_disj:
-  ∀A B p. clkfree_q A ∧ clkfree_q B ⇒ (∀s. wp p (λ(r,t). A (r,t) ∨ B (r,t)) s ⇔ wp p A s ∨ wp p B s)
-Proof
-  rw[wp_def]
-  >> iff_tac
-  >> rw[]
-  >- (pairarg_tac >> gvs[]
-      >- (disj1_tac >> qexists ‘k’ >> gvs[])
-      >- (disj2_tac >> qexists ‘k’ >> gvs[]))
-  >- metis_tac[clkfree_q_disj]
-  >- (qexists ‘k’ >> pairarg_tac >> gvs[])
-  >- metis_tac[clkfree_q_disj]
-  >> qexists ‘k’
   >> pairarg_tac
   >> gvs[]
 QED
 
-Theorem wp_neg:
-  ∀A p. clkfree_q A ⇒ (∀s. wp p (λ(r,t). ¬A (r,t)) s ⇒ ¬wp p A s)
+Theorem wp_disj:
+  ∀A B p s. wp p (λ(r,t). A (r,t) ∨ B (r,t)) s ⇔ wp p A s ∨ wp p B s
 Proof
   rw[wp_def]
+  >> iff_tac
   >> rw[]
-  >> rpt (pairarg_tac >> gvs[])
-  >> Cases_on ‘k > k'’
-  >- (qspecl_then [‘p’, ‘s with clock := k'’, ‘r’, ‘t’, ‘k - k'’]
-                   assume_tac evaluate_add_clock_eq
-      >> elim_cases [‘r = SOME TimeOut’]
-      >> gvs[clkfree_q_def]
-      >> first_x_assum $ (qspecl_then [‘r’, ‘t’, ‘t.clock’, ‘k + t.clock - k'’] assume_tac)
-      >> gvs[state_clock_idem])
-  >- (qspecl_then [‘p’, ‘s with clock := k’, ‘r'’, ‘t'’, ‘k' - k’]
-                   assume_tac evaluate_add_clock_eq
-      >> gvs[clkfree_q_def]
-      >> first_x_assum $ (qspecl_then [‘r’, ‘t'’, ‘t'.clock’, ‘k' + t'.clock - k’] assume_tac)
-      >> gvs[state_clock_idem])
+  >> pairarg_tac
+  >> gvs[]
 QED
 
 Theorem wp_nif:
-  ∀Q M p res. clkfree_q Q ∧ clkfree_p M ⇒
-              (∀s. wp p (λ(r,t). if r ≠ res then Q (r,t) else M t) s ⇔
-                   wp p (λ(r,t). r ≠ res ∧ Q (r,t)) s ∨ wp p (λ(r,t). r = res ∧ M t) s)
+  ∀Q M p res s. wp p (λ(r,t). if r ≠ res then Q (r,t) else M t) s ⇔
+                wp p (λ(r,t). r ≠ res ∧ Q (r,t)) s ∨ wp p (λ(r,t). r = res ∧ M t) s
 Proof
   rw[wp_def]
   >> iff_tac
   >> rw[]
-  >> rpt (pairarg_tac >> gvs[])
-  >> gvs[clkfree_qnif]
-  >| [Cases_on ‘r ≠ res’ >> gvs[] >| [disj1_tac, disj2_tac] >> rw[], ALL_TAC, ALL_TAC]
-  >> gvs[clkfree_qqn,clkfree_pq]
-  >> qexists ‘k’
+  >> pairarg_tac
+  >> gvs[]
+  >> Cases_on ‘r ≠ res’
   >> gvs[]
 QED
-
+        
 Theorem wp_skip:
-  clkfree_q Q ⇒ (wp Skip Q s ⇔ Q (NONE, s))
+  wp Skip Q s ⇔ Q (NONE, s)
 Proof
-  rw[wp_def,evaluate_def,clkfree_q_def]
-  >> assume_tac state_clock_idem
-  >> iff_tac
-  >> rw[]
-  >- (first_x_assum $ (qspecl_then [‘NONE’, ‘s’, ‘k’, ‘s.clock’] assume_tac) >> gvs[])
-  >> qexists ‘s.clock’
-  >> gvs[]
+  rw[wp_def,evaluate_def]
 QED
 
 Theorem wp_dec:
-  clkfree_q Q ⇒ (wp (Dec v sh src prog) Q s ⇔ evaluates src s ∧
-                                              subst Local v src (wp prog (reset_subst v s Q)) s)
+  wp (Dec v sh src prog) Q s ⇔ evaluates src s ∧
+                               subst Local v src (wp prog (reset_subst v s Q)) s
 Proof
-  rw[wp_def,evaluate_def,clkfree_q_def,evaluates_def,subst_def,reset_subst_def]
+  rw[wp_def,evaluate_def,evaluates_def,subst_def,reset_subst_def]
   >> iff_tac
   >> rw[]
-  >> assume_tac state_clock_idem
-  >> assume_tac eval_upd_clock_eq
-  >> elim_cases [‘eval s src’]
-  >> rpt (pairarg_tac >> gvs[])
-  >> rw[]
-  >- (first_x_assum $ (qspecl_then [‘r'’,
-                                    ‘s' with locals := res_var s'.locals (v,FLOOKUP s.locals v)’,
-                                    ‘k1’, ‘k2’] assume_tac)
-      >> gvs[])
-  >> qexists ‘k’
+  >> rpt(pairarg_tac >> gvs[])
+  >> FULL_CASE_TAC
+  >> gvs[]
+  >> pairarg_tac
   >> gvs[]
 QED
 
 Theorem wp_assign:
-  clkfree_q Q ⇒ (wp (Assign k v src) Q s ⇔ valid_value k v src s ∧
-                                           subst k v src (λs. Q (NONE, s)) s)
+  wp (Assign k v src) Q s ⇔ valid_value k v src s ∧
+                            subst k v src (λs. Q (NONE, s)) s
 Proof
   Cases_on ‘k’
-  >> rw[wp_def,evaluate_def,clkfree_q_def,valid_value_def,subst_def]
+  >> rw[wp_def,evaluate_def,valid_value_def,subst_def]
   >> iff_tac
   >> rw[]
-  >> assume_tac state_clock_idem
-  >> assume_tac eval_upd_clock_eq
-  >> elim_cases [‘eval s src’]
-  >- elim_cases [‘is_valid_value s.locals v x’]
-  >- (elim_cases [‘is_valid_value s.locals v x’]
-      >> first_x_assum $ (qspecl_then [‘NONE’, ‘s with locals := s.locals |+ (v,x)’,
-                                       ‘k’, ‘s.clock’] assume_tac)
-      >> gvs[])
-  >- (qexists ‘s.clock’ >> gvs[])
-  >- elim_cases [‘is_valid_value s.globals v x’]
-  >- (elim_cases [‘is_valid_value s.globals v x’]
-      >> first_x_assum $ (qspecl_then [‘NONE’, ‘s with globals := s.globals |+ (v,x)’,
-                                       ‘k’, ‘s.clock’] assume_tac)
-      >> gvs[])
-  >> qexists ‘s.clock’
+  >> pairarg_tac
   >> gvs[]
+  >> rpt(FULL_CASE_TAC >> gvs[])
 QED
 
 Theorem wp_store:
-  clkfree_q Q ⇒ (wp (Store dest src) Q s ⇔ ∃addr val. evaluates_to dest (ValWord addr) s ∧
-                                                      evaluates_to src val s ∧
-                                                      addr_in_mem addr val s ∧
-                                                      mem_subst addr val (λs. Q (NONE, s)) s)
+  wp (Store dest src) Q s ⇔ ∃addr val. evaluates_to dest (ValWord addr) s ∧
+                                       evaluates_to src val s ∧
+                                       addr_in_mem addr val s ∧
+                                       mem_subst addr val (λs. Q (NONE, s)) s
 Proof
-  rw[wp_def,evaluate_def,clkfree_q_def,evaluates_to_def,addr_in_mem_def,mem_subst_def]
+  rw[wp_def,evaluate_def,evaluates_to_def,addr_in_mem_def,mem_subst_def]
   >> iff_tac
   >> rw[]
-  >> assume_tac state_clock_idem
-  >> assume_tac eval_upd_clock_eq
-  >> elim_cases [‘eval s src’, ‘eval s dest’]
-  >- elim_cases [‘x’]
-  >- (elim_cases [‘x'’, ‘w’, ‘mem_stores c (flatten x) s.memaddrs s.memory’]
-      >> first_x_assum $ (qspecl_then [‘NONE’, ‘s with memory := x'’,
-                                       ‘k’, ‘s.clock’] assume_tac)
-      >> gvs[])
-  >> qexists ‘s.clock’
+  >> pairarg_tac
   >> gvs[]
+  >> rpt (FULL_CASE_TAC >> gvs[])
 QED
 
 Theorem wp_store32:
-  clkfree_q Q ⇒ (wp (Store32 dest src) Q s ⇔ ∃addr val. evaluates_to dest (ValWord addr) s ∧
-                                                        evaluates_to src (ValWord val) s ∧
-                                                        addr_in_mem_32 addr val s ∧
-                                                        mem_subst_32 addr val (λs. Q (NONE, s)) s)
+  wp (Store32 dest src) Q s ⇔ ∃addr val. evaluates_to dest (ValWord addr) s ∧
+                                         evaluates_to src (ValWord val) s ∧
+                                         addr_in_mem_32 addr val s ∧
+                                         mem_subst_32 addr val (λs. Q (NONE, s)) s
 Proof
-  rw[wp_def,evaluate_def,clkfree_q_def,evaluates_to_def,addr_in_mem_32_def,mem_subst_32_def]
+  rw[wp_def,evaluate_def,evaluates_to_def,addr_in_mem_32_def,mem_subst_32_def]
   >> iff_tac
   >> rw[]
-  >> assume_tac state_clock_idem
-  >> assume_tac eval_upd_clock_eq
-  >> elim_cases [‘eval s src’, ‘eval s dest’]
-  >- elim_cases [‘x’]
-  >- (elim_cases [‘x’, ‘x'’, ‘w’, ‘w'’, ‘mem_store_32 s.memory s.memaddrs s.be c' (w2w c)’]
-      >> first_x_assum $ (qspecl_then [‘NONE’, ‘s with memory := x’,
-                                       ‘k’, ‘s.clock’] assume_tac)
-      >> gvs[])
-  >> qexists ‘s.clock’
+  >> pairarg_tac
   >> gvs[]
+  >> rpt (FULL_CASE_TAC >> gvs[])
 QED
 
 Theorem wp_storebyte:
-  clkfree_q Q ⇒ (wp (StoreByte dest src) Q s ⇔ ∃addr val. evaluates_to dest (ValWord addr) s ∧
-                                                          evaluates_to src (ValWord val) s ∧
-                                                          addr_in_mem_byte addr val s ∧
-                                                          mem_subst_byte addr val (λs. Q (NONE, s)) s)
+  wp (StoreByte dest src) Q s ⇔ ∃addr val. evaluates_to dest (ValWord addr) s ∧
+                                           evaluates_to src (ValWord val) s ∧
+                                           addr_in_mem_byte addr val s ∧
+                                           mem_subst_byte addr val (λs. Q (NONE, s)) s
 Proof
-  rw[wp_def,evaluate_def,clkfree_q_def,evaluates_to_def,addr_in_mem_byte_def,mem_subst_byte_def]
+  rw[wp_def,evaluate_def,evaluates_to_def,addr_in_mem_byte_def,mem_subst_byte_def]
   >> iff_tac
   >> rw[]
-  >> assume_tac state_clock_idem
-  >> assume_tac eval_upd_clock_eq
-  >> elim_cases [‘eval s src’, ‘eval s dest’]
-  >- elim_cases [‘x’]
-  >- (elim_cases [‘x’, ‘x'’, ‘w’, ‘w'’, ‘mem_store_byte s.memory s.memaddrs s.be c' (w2w c)’]
-      >> first_x_assum $ (qspecl_then [‘NONE’, ‘s with memory := x’,
-                                       ‘k’, ‘s.clock’] assume_tac)
-      >> gvs[])
-  >> qexists ‘s.clock’
+  >> pairarg_tac
   >> gvs[]
+  >> rpt (FULL_CASE_TAC >> gvs[])
 QED
 
 Theorem wp_seq:
-  clkfree_q Q ⇒ (wp (Seq p1 p2) Q s ⇔ wp p1 (λ(r,t). r = NONE ∧ (wp p2 Q) t) s ∨
-                                      wp p1 (λ(r,t). r ≠ NONE ∧ Q (r,t)) s)
+  wp (Seq p1 p2) Q s ⇔ wp p1 (λ(r,t). r = NONE ∧ (wp p2 Q) t) s ∨
+                       wp p1 (λ(r,t). r ≠ NONE ∧ Q (r,t)) s
 Proof
-  rw[wp_def,evaluate_def,clkfree_q_def]
+  rw[wp_def,evaluate_def]
   >> iff_tac
   >> rw[]
   >> rpt (pairarg_tac >> gvs[])
-  >- (Cases_on ‘res’
-      >> gvs[]
-      >- (disj1_tac
-          >> qspecl_then [‘s with clock := k’, ‘s1’, ‘NONE’, ‘p1’]
-                         assume_tac (GEN_ALL evaluate_min_clock)
-          >> gvs[]
-          >> qexists ‘k' + s1.clock’
-          >> rpt (pairarg_tac >> gvs[])
-          >> qspecl_then [‘p1’, ‘s with clock := k'’, ‘NONE’, ‘s1 with clock := 0’, ‘s1.clock’]
-                         assume_tac evaluate_add_clock_eq
-          >> gvs[]
-          >> qexists ‘s1.clock’
-          >> gvs[state_clock_idem])
-      >> disj2_tac
-      >> rw[]
-      >- (first_x_assum $ (qspecl_then [‘r’, ‘s'’, ‘k1’, ‘k2’] assume_tac) >> gvs[])
-      >> qexists ‘k’
-      >> gvs[])
-  >- (qspecl_then [‘s with clock := k’, ‘t’, ‘NONE’, ‘p1’]
-                  assume_tac (GEN_ALL evaluate_min_clock)
-      >> gvs[]
-      >> qexists ‘k'' + k'’
-      >> qspecl_then [‘p1’, ‘s with clock := k''’, ‘NONE’, ‘t with clock := 0’, ‘k'’]
-                     assume_tac evaluate_add_clock_eq
-      >> gvs[])
-  >> qexists ‘k’
+  >> FULL_CASE_TAC
   >> gvs[]
 QED
 
 Theorem wp_if:
-  clkfree_q Q ⇒ (wp (If e c1 c2) Q s ⇔ (evaluates_to_word  e s)             ∧
-                                       (evaluates_to_true  e s ⇒ wp c1 Q s) ∧
-                                       (evaluates_to_false e s ⇒ wp c2 Q s))
+  wp (If e c1 c2) Q s ⇔ (evaluates_to_word  e s)             ∧
+                        (evaluates_to_true  e s ⇒ wp c1 Q s) ∧
+                        (evaluates_to_false e s ⇒ wp c2 Q s)
 Proof
   rw[wp_def,evaluate_def,evaluates_to_word_def,evaluates_to_true_def,evaluates_to_false_def]
   >> iff_tac
   >> rw[]
-  >> assume_tac eval_upd_clock_eq
-  >- elim_cases [‘eval s e’, ‘x’, ‘w’]
-  >- (qexists ‘k’ >> gvs[])
-  >> elim_cases [‘w = 0w’]
-  >> qexists ‘k’
+  >> pairarg_tac
   >> gvs[]
+  >> rpt (FULL_CASE_TAC >> gvs[])
 QED
 
 Theorem wp_break:
-  clkfree_q Q ⇒ (wp Break Q s ⇔ Q (SOME Break,s))
+  wp Break Q s ⇔ Q (SOME Break,s)
 Proof
-  rw[wp_def,evaluate_def,clkfree_q_def]
-  >> assume_tac state_clock_idem
-  >> iff_tac
-  >> rw[]
-  >- (first_x_assum $ (qspecl_then [‘SOME Break’, ‘s’, ‘k’, ‘s.clock’] assume_tac) >> gvs[])
-  >> qexists ‘s.clock’
-  >> gvs[]
+  rw[wp_def,evaluate_def]
 QED
 
 Theorem wp_continue:
-  clkfree_q Q ⇒ (wp Continue Q s ⇔ Q (SOME Continue,s))
+  wp Continue Q s ⇔ Q (SOME Continue,s)
 Proof
-  rw[wp_def,evaluate_def,clkfree_q_def]
-  >> assume_tac state_clock_idem
-  >> iff_tac
-  >> rw[]
-  >- (first_x_assum $ (qspecl_then [‘SOME Continue’, ‘s’, ‘k’, ‘s.clock’] assume_tac) >> gvs[])
-  >> qexists ‘s.clock’
-  >> gvs[]
+  rw[wp_def,evaluate_def]
 QED
 
 Theorem wp_raise:
-  clkfree_q Q ⇒ (wp (Raise eid e) Q s ⇔ ∃sh val. has_eshape eid sh s ∧
-                                                 evaluates_to e val s ∧
-                                                 shape_of val = sh ∧
-                                                 size_of_shape sh ≤ 32 ∧
-                                                 Q (SOME (Exception eid val),empty_locals s))
+  wp (Raise eid e) Q s ⇔ ∃sh val. has_eshape eid sh s ∧
+                                  evaluates_to e val s ∧
+                                  shape_of val = sh ∧
+                                  size_of_shape sh ≤ 32 ∧
+                                  Q (SOME (Exception eid val),empty_locals s)
 Proof
-  rw[wp_def,evaluate_def,clkfree_q_def,has_eshape_def,evaluates_to_def]
+  rw[wp_def,evaluate_def,has_eshape_def,evaluates_to_def]
   >> iff_tac
   >> rw[]
   >> rpt (pairarg_tac >> gvs[])
-  >> assume_tac state_clock_idem
-  >> assume_tac eval_upd_clock_eq
-  >- (elim_cases [‘FLOOKUP s.eshapes eid’, ‘eval s e’, ‘shape_of x' = x’,
-                  ‘size_of_shape (shape_of x') ≤ 32’]
-      >> first_x_assum $ (qspecl_then [‘SOME (Exception eid x')’, ‘s with locals := FEMPTY’,
-                                       ‘s.clock’, ‘k’] assume_tac)
-      >> gvs[empty_locals_def])
-  >> qexists ‘s.clock’
-  >> gvs[]
+  >> rpt (FULL_CASE_TAC >> gvs[])
 QED
 
 Theorem wp_return:
-  clkfree_q Q ⇒ (wp (Return e) Q s ⇔ ∃val. evaluates_to e val s ∧
-                                           size_of_shape (shape_of val) ≤ 32 ∧
-                                           Q (SOME (Return val),empty_locals s))
+  wp (Return e) Q s ⇔ ∃val. evaluates_to e val s ∧
+                            size_of_shape (shape_of val) ≤ 32 ∧
+                            Q (SOME (Return val),empty_locals s)
 Proof
-  rw[wp_def,evaluate_def,clkfree_q_def,evaluates_to_def]
+  rw[wp_def,evaluate_def,evaluates_to_def]
   >> iff_tac
   >> rw[]
   >> rpt (pairarg_tac >> gvs[])
-  >> assume_tac state_clock_idem
-  >> assume_tac eval_upd_clock_eq
-  >- (elim_cases [‘eval s e’, ‘size_of_shape (shape_of x) ≤ 32’]
-      >> first_x_assum $ (qspecl_then [‘SOME (Return x)’, ‘s with locals := FEMPTY’,
-                                       ‘s.clock’, ‘k’] assume_tac)
-      >> gvs[empty_locals_def])
-  >> qexists ‘s.clock’
-  >> gvs[]
+  >> rpt (FULL_CASE_TAC >> gvs[])
 QED
 
 Theorem wp_annot:
-  clkfree_q Q ⇒ (wp (Annot a b) Q s ⇔ Q (NONE,s))
+  wp (Annot a b) Q s ⇔ Q (NONE,s)
 Proof
-  rw[wp_def,evaluate_def,clkfree_q_def]
-  >> assume_tac state_clock_idem
-  >> iff_tac
-  >> rw[]
-  >- (first_x_assum $ (qspecl_then [‘NONE’, ‘s’, ‘k’, ‘s.clock’] assume_tac) >> gvs[])
-  >> qexists ‘s.clock’
-  >> gvs[]
+  rw[wp_def,evaluate_def]
 QED
